Extremely messy, but trying out new things.

examples/lists/list-utils.dfy
@@ -4,6 +4,7 @@ Some useful list-related definitions, including:
   - Common functions on lists
   - Definitions for decomposing cons-lists and concatenation lists.
   - Coding functions between list types 
+  - Representation function
 */
 
 module Lists {
@@ -36,6 +37,13 @@ module Lists {
     case Conc(x, y) => "(" + PrintListC(x) + ", " + PrintListC(y) + ")" 
   }
 
+  function method ListConc(a: List, b: List): List 
+  {
+    match a 
+    case Nil => b 
+    case Cons(head, tail) => Cons(head, ListConc(tail, b))
+  }
+
   // Note the special case for x == NilC 
   function method AssociateLeft(x: ListC, a: int, y: ListC): ListC
   {
@@ -43,6 +51,7 @@ module Lists {
   }
 
   function method AssociateRight(x: ListC, a: int, y: ListC): ListC 
+    // ensures Rep(AssociateRight(x, a, y)) == 
   {
     if x == NilC then Conc(El(a), y) else Conc(x, Conc(El(a), y))
   }
@@ -94,34 +103,125 @@ module Lists {
     case Cons(a, x) => Conc(El(a), SimpleCoding(x))
   }
 
-  function method Aux(orig: List, right: List, x: ListC, a: int, y: ListC): set<ListC> 
-    decreases y 
-    requires SimpleCoding(right) == Conc(El(a), y) 
-    requires y != NilC ==> y.Conc? 
-    requires y != NilC ==> y.left.El? // specifies the structure of y
-    ensures forall t: ListC :: (t in Aux(orig, right, x, a, y)) ==> t.Conc?
+  // function method Aux(orig: List, right: List, x: ListC, a: int, y: ListC): set<ListC> 
+  //   decreases y 
+  //   requires SimpleCoding(right) == Conc(El(a), y) 
+  //   requires Rep(AssociateRight(x, a, y)) == orig
+  //   requires y != NilC ==> y.Conc? 
+  //   requires y != NilC ==> y.left.El? // specifies the structure of y
+  //   requires x.Conc? ==> InitDecomposableC(x)
+  //   requires x == NilC ==> Conc(El(a), y) == SimpleCoding(orig)
+  //   ensures forall t: ListC :: (t in Aux(orig, right, x, a, y)) ==> t.Conc?
+  //   ensures forall t: ListC :: (t in Aux(orig, right, x, a, y)) ==> (t.left.Conc? ==> InitDecomposableC(t.left))
+  //   ensures forall t: ListC :: (t in Aux(orig, right, x, a, y)) ==> t.left != NilC
+  //   ensures AssociateLeft(x, a, y) in Aux(orig, right, x, a, y) ==> AssociateRight(x, a, y) in Aux(orig, right, x, a, y)
+  //   ensures Rep(AssociateRight(x, a, y)) == orig
+  // {
+  //   RepInvariant(x, a, y);
+  //   // assume Rep(AssociateRight(x, a, y)) == orig;
+  //   if y == NilC then {AssociateRight(x, a, y)}
+  //                else Aux(orig, right.tail, if x == NilC then El(a) else Conc(x, El(a)), y.left.val, y.right) + {AssociateRight(x, a, y)}
+  // }
+
+  // function method ComplexCoding(l: List): set<ListC>
+  //   ensures l != Nil ==> forall t: ListC :: t in ComplexCoding(l) ==> t.Conc?
+  //   ensures l != Nil ==> forall t: ListC :: (t in ComplexCoding(l) && t.Conc? && t.left.Conc?) ==> InitDecomposableC(t.left)
+  //   // ensures forall x: ListC, a: int, y: ListC :: AssociateLeft(x, a, y) in ComplexCoding(l) ==> AssociateRight(x, a, y) in ComplexCoding(l)
+  // {
+  //   assume l.Cons? ==> Rep(AssociateRight(NilC, l.head, SimpleCoding(l.tail))) == l;
+  //   if l == Nil then {NilC} else Aux(l, l, NilC, l.head, SimpleCoding(l.tail))
+  // }
+
+  function method NewAux(x: ListC, y: List): set<ListC> 
+    decreases y
+    ensures forall t: ListC :: t in NewAux(x, y) ==> t.Conc?
   {
-    if y == NilC then {AssociateRight(x, a, y)}
-                 else Aux(orig, right.tail, if x == NilC then El(a) else Conc(x, El(a)), y.left.val, y.right) + {AssociateRight(x, a, y)}
+    match y 
+    case Nil => {} 
+    case Cons(head, tail) => NewAux(Conc(x, El(head)), tail) + {Conc(x, SimpleCoding(y))}
+    // {Conc(Conc(x, El(head)), SimpleCoding(tail))}
+    //{AssociateLeft(x, head, SimpleCoding(y))}
   }
 
-  function ComplexCoding(l: List): set<ListC>
+  function method NewComplex(l: List): set<ListC> 
   {
-    if l == Nil then {NilC} else Aux(l, l, NilC, l.head, SimpleCoding(l.tail))
+    NewAux(NilC, l) // maybe instead El(l.head), l.tail?
+  }
+
+  /**** ListC -> List representation function ****/
+  function method Rep(x: ListC): List 
+  {
+    match x
+    case NilC => Nil 
+    case El(a) => Cons(a, Nil) 
+    case Conc(a, b) => ListConc(Rep(a), Rep(b))
+    // if Rep(a) == Nil then Rep(b) else Rep(a).(tail := Rep(b)) // datatype update syntax 
+  }
+
+  //
+
+  // Rep is a left inverse of SimpleCoding 
+  lemma SimpleRepInverse(l: List, x: ListC)
+    requires x == SimpleCoding(l)
+    ensures Rep(x) == l
+  {
+    assume Rep(x) == l;
+  }
+
+  lemma ListConcAssoc(x: List, y: List, z: List)
+    ensures ListConc(ListConc(x, y), z) == ListConc(x, ListConc(y, z))
+  {
+    // match x 
+    // case Nil => {} 
+    // case Cons(x_head, x_tail) => {
+    //   match y 
+    //   case Nil => {}
+    //   case Cons(y_head, y_tail) => {
+    //     match z
+    //     case Nil => {
+    //       assert ListConc(ListConc(x, y), z) == ListConc(x, y);
+    //     } 
+    //     case Cons(z_head, z_tail) => {}
+    //   }
+    // }
+  }
+
+  lemma AssocRepEquiv(x: ListC, y: ListC, z: ListC)
+    ensures Rep(Conc(Conc(x, y), z)) == Rep(Conc(x, Conc(y, z)))
+  {
+    ListConcAssoc(Rep(x), Rep(y), Rep(z));
+  }
+
+  lemma RepInverse(l: List, x: ListC) 
+    decreases x.left
+    requires x in NewComplex(l)
+    ensures Rep(x) == l
+  {
+    if x == Conc(NilC, SimpleCoding(l)) {
+      SimpleRepInverse(l, SimpleCoding(l));
+    }
+    else {
+      assume x.left.Conc?;
+      assume InitDecomposableC(x.left);
+      assume Conc(x.left.left, Conc(x.left.right, x.right)) in NewComplex(l);
+      RepInverse(l, Conc(x.left.left, Conc(x.left.right, x.right)));
+      AssocRepEquiv(x.left.left, x.left.right, x.right);
+    }
   }
 
   // Sanity check
-  // method Main() {
-  //   var l := Cons(5, Cons(-2, Cons(3, Cons(-2, Cons(3, Nil)))));
-  //   var assoc := ComplexCoding(l);
-  //   var c := assoc;
-  //   while c != {} 
-  //     decreases c;
-  //   {
-  //     var y :| y in c;
-  //     print PrintListC(y) + "\n";
-  //     c := c - { y };
-  //   }
-  // }
+  method Main() {
+    var l := Cons(5, Cons(-2, Cons(3, Cons(-2, Cons(3, Nil)))));
+    // var assoc := ComplexCoding(l);
+    var assoc := NewComplex(l);
+    var c := assoc;
+    while c != {} 
+      decreases c;
+    {
+      var y :| y in c;
+      print PrintListC(y) + "\n";
+      c := c - { y };
+    }
+  }
 
 }
