examples/lists/max-tail-sum-rep-function-testing.dfy
@@ -1,0 +1,107 @@
+/*
+Here we try the maximum tail sum example of recsynt Section A.1.3.
+We use a coding function that changes up the recursive structure of the list. 
+We try to explicitly produce a set of lists with the coding function.
+WARNING: messy and does not verify. 
+*/
+
+include "./list-utils.dfy"
+module MaxTailSum {
+  import opened Lists
+  function method Max(x: int, y: int): int 
+  {
+    if x < y then y else x
+  }
+
+  // Sequential (leftwards). 
+  // Note that the function is already lifted.
+  function method F(l: List): (int, int) 
+  {
+    match l 
+    case Nil => (0, 0)
+    case Cons(a, x) => FoldOp(a, F(x))
+  }
+
+  // Operator given as input to the fold
+  function method FoldOp(a: int, res: (int, int)): (int, int)
+  {
+    var (s, m) := res; // (sum, max)
+    (s + a, Max(m, s + a))
+  }
+
+  function method MainF(l: List): (int, int)
+  {
+    F(l)
+  }
+
+  // Homomorphism. 
+  function method G(l: ListC): (int, int) 
+    ensures G(l).1 >= G(l).0
+  {
+    match l 
+    case NilC => (0, 0)
+    case El(a) => (a, Max(a, 0)) 
+    case Conc(x, y) => Join(G(x), G(y))
+  }
+
+  function method Join(res1: (int, int), res2: (int, int)): (int, int)
+    // ensures Join(res1, res2).1 == res1.1
+  {
+    var (s1, m1), (s2, m2) := res1, res2;
+    (s1 + s2, Max(s2 + m1, m2))
+  }
+
+  function method MainG(l: ListC): (int, int)
+    ensures MainG(l).1 >= MainG(l).0
+  {
+    G(l)
+  }
+
+
+  /**** Some experiments with the Rep function ****/
+  lemma RepInverse(l: List, x: ListC) 
+    requires x in NewComplex(l)
+    ensures Rep(x) == l
+  {
+    // match l 
+    // case Nil => {} 
+    // case Cons(head, tail) => {
+
+    // }
+    assume Rep(x) == l;
+  }
+
+  
+
+  lemma FHom(x: List, y: List) 
+    ensures MainF(ListConc(x, y)) == Join(MainF(x), MainF(y))
+  {
+    assume MainF(ListConc(x, y)) == Join(MainF(x), MainF(y));
+  }
+
+
+  lemma FRepBehaviour(x: ListC) 
+    ensures MainG(x) == MainF(Rep(x))
+  {
+    match x 
+    case NilC => {}
+    case El(a) => {
+      assert F(Nil) == (0, 0);
+    }
+    case Conc(a, b) => {
+      FHom(Rep(a), Rep(b));
+    }
+  }
+
+  lemma EquivalentSchemes(l: List, x: ListC)
+    requires x in NewComplex(l)
+    ensures MainF(l) == MainG(x) 
+  {
+    RepInverse(l, x);
+    FRepBehaviour(x);
+  }
+}
+
+
+
+
